src/program_proof/tulip/program/replica/replica_commit.v
@@ -12,13 +12,14 @@ Section program.
     (rp : loc) (tsW : u64) (pwrsS : Slice.t) (pwrs : dbmap) gid rid γ :
     let ts := uint.nat tsW in
     safe_commit γ gid ts pwrs -∗
+    is_dbmap_in_slice pwrsS pwrs -∗
     is_replica_plus_txnlog rp gid rid γ -∗
-    {{{ own_dbmap_in_slice pwrsS pwrs }}}
+    {{{ True }}}
       Replica__Commit #rp #tsW (to_val pwrsS)
     {{{ (ok : bool), RET #ok; True }}}.
   Proof.
-    iIntros (ts) "#Hsafe #Hrp".
-    iIntros (Φ) "!> Hpwrs HΦ".
+    iIntros (ts) "#Hsafe #Hpwrs #Hrp".
+    iIntros (Φ) "!> _ HΦ".
     wp_rec.
 
     (*@ func (rp *Replica) Commit(ts uint64, pwrs []tulip.WriteEntry) bool {    @*)
@@ -45,7 +46,7 @@ Section program.
     (*@                                                                         @*)
     iNamed "Hrp". iNamed "Htxnlog".
     wp_loadField.
-    wp_apply (wp_TxnLog__SubmitCommit with "Htxnlog Hpwrs").
+    wp_apply (wp_TxnLog__SubmitCommit with "Hpwrs Htxnlog").
     iNamed "Hinv".
     iInv "Hinv" as "> HinvO" "HinvC".
     iNamed "HinvO".
