src/program_proof/tulip/program/replica/replica_inquire.v
@@ -1,0 +1,276 @@
+From Perennial.program_proof.tulip.invariance Require Import execute advance.
+From Perennial.program_proof.tulip.program Require Import prelude.
+From Perennial.program_proof.tulip.program.replica Require Import
+  replica_repr replica_finalized replica_lowest_rank replica_validated
+  replica_last_proposal replica_advance replica_log.
+
+Section program.
+  Context `{!heapGS Σ, !tulip_ghostG Σ}.
+
+  Theorem wp_Replica__inquire
+    (rp : loc) (tsW : u64) (rankW : u64) (cid : coordid) gid rid γ α :
+    let ts := uint.nat tsW in
+    let rank := uint.nat rankW in
+    gid ∈ gids_all ->
+    rid ∈ rids_all ->
+    valid_ts ts ->
+    valid_backup_rank rank ->
+    know_tulip_inv γ -∗
+    know_replica_file_inv γ gid rid -∗
+    {{{ own_replica rp gid rid γ α }}}
+      Replica__inquire #rp #tsW #rankW
+    {{{ (pp : ppsl) (vd : bool) (pwrsP : Slice.t) (res : rpres) (pwrs : dbmap),
+          RET (ppsl_to_val pp, #vd, to_val pwrsP, #(rpres_to_u64 res)); 
+        own_replica rp gid rid γ α ∗
+        inquire_outcome γ gid rid cid ts rank (uint.nat pp.1) pp.2 vd pwrs res ∗
+        if vd then is_dbmap_in_slice pwrsP pwrs else True
+    }}}.
+  Proof.
+    iIntros (ts rank Hgid Hrid Hvts Hvrank) "#Hinv #Hinvfile".
+    iIntros (Φ) "!> Hrp HΦ".
+    wp_rec.
+
+    (*@ func (rp *Replica) inquire(ts uint64, rank uint64) (tulip.PrepareProposal, bool, []tulip.WriteEntry, uint64) { @*)
+    (*@     // Check if the transaction has aborted or committed. If so, returns the @*)
+    (*@     // status immediately.                                              @*)
+    (*@     res, done := rp.finalized(ts)                                       @*)
+    (*@     if done {                                                           @*)
+    (*@         return tulip.PrepareProposal{}, false, nil, res                 @*)
+    (*@     }                                                                   @*)
+    (*@                                                                         @*)
+    wp_pures.
+    wp_apply (wp_Replica__finalized with "Hinv Hrp").
+    { apply Hgid. }
+    iIntros (res final) "[Hrp Hres]".
+    wp_pures.
+    destruct final; wp_pures.
+    { iModIntro.
+      iApply ("HΦ" $! (W64 0, false) false Slice.nil res ∅).
+      iFrame "Hrp".
+      iSplit; last done.
+      by destruct res.
+    }
+
+    (*@     // Check if @rank is still available. Note the difference between this @*)
+    (*@     // method and @tryAccept: The case where @rank = @ps.rankl indicates another @*)
+    (*@     // replica's attempt to become the coordinator at @rank, which should be @*)
+    (*@     // rejected. Note the rank setup: rank 0 and 1 are reserved for the client @*)
+    (*@     // (similarly to Paxos's ballot assignment), and the others are contended by @*)
+    (*@     // replicas (similarly to Raft's voting process).                   @*)
+    (*@     rankl, ok := rp.lowestRank(ts)                                      @*)
+    (*@     if ok && rank <= rankl {                                            @*)
+    (*@         return tulip.PrepareProposal{}, false, nil, tulip.REPLICA_STALE_COORDINATOR @*)
+    (*@     }                                                                   @*)
+    (*@                                                                         @*)
+    do 2 iNamed "Hrp".
+    wp_apply (wp_Replica__lowestRank with "Hpsmrkm").
+    iIntros (rankl ok) "[Hpsmrkm %Hrankl]".
+    wp_pures.
+    unshelve wp_apply (wp_and_pure (ok = true)).
+    { shelve. }
+    { apply _. }
+    { shelve. }
+    { wp_pures. case_bool_decide as Hcase; last apply not_true_is_false in Hcase; by subst ok. }
+    { iIntros (_). by wp_pures. }
+    case_bool_decide as Hadvanced; wp_pures.
+    { iApply ("HΦ" $! (W64 0, false) false Slice.nil ReplicaStaleCoordinator ∅).
+      by iFrame "∗ # %".
+    }
+
+    (*@     // Note that in the case where the fast path is not taken (i.e., @ok = @*)
+    (*@     // false), we want (0, false), which happens to be the zero-value.  @*)
+    (*@     ranka, pdec, _ := rp.lastProposal(ts)                               @*)
+    (*@     pp := tulip.PrepareProposal{ Rank: ranka, Prepared: pdec }          @*)
+    (*@                                                                         @*)
+    wp_apply (wp_Replica__lastProposal with "Hpsmrkm").
+    iIntros (ranka pdec ex) "[Hpsmrkm %Hex]".
+
+    (*@     // Update the lowest acceptable rank.                               @*)
+    (*@     // Logical action: Advance lowest acceptable rank of @ts to @rank.  @*)
+    (*@     rp.advance(ts, rank)                                                @*)
+    (*@                                                                         @*)
+    wp_apply (wp_Replica__advance with "Hpsmrkm").
+    iIntros "Hpsmrkm".
+
+    (*@     // Create an inconsistent log entry.                                @*)
+    (*@     logAdvance(rp.fname, rp.lsna, ts, rank)                             @*)
+    (*@                                                                         @*)
+    wp_pures.
+    iNamed "Hlsna".
+    wp_loadField.
+    iNamed "Hfname".
+    wp_loadField.
+    wp_apply wp_logAdvance.
+    (* Open the crash, replica, and file invariants. *)
+    iMod (own_crash_ex_open with "Hdurable") as "[> Hdurable HdurableC]".
+    { solve_ndisj. }
+    iNamed "Hdurable".
+    iNamed "Hinv".
+    iInv "Hinv" as "> HinvO" "HinvC".
+    iInv "Hinvfile" as "> HinvfileO" "HinvfileC".
+    iNamed "HinvfileO".
+    (* Agree on the fname, and merge the two ilog quarter. *)
+    iDestruct (replica_ilog_fname_agree with "Hfname Hilogfname") as %->.
+    iDestruct (replica_ilog_combine with "Hilog Hilogfileinv") as "[Hilog ->]".
+    iApply ncfupd_mask_intro; first solve_ndisj.
+    iIntros "Hmask".
+    (* Give the file points-to to the logging method. *)
+    iFrame "Hfile %".
+    iIntros (bs' failed) "Hfile".
+    destruct failed.
+    { (* Case: Write failed. Close the invariants without any updates. *)
+      iMod "Hmask" as "_".
+      iDestruct (replica_ilog_split with "Hilog") as "[Hilog Hilogfileinv]".
+      iMod ("HinvfileC" with "[Hfile Hilogfileinv]") as "_".
+      { by iFrame "∗ # %". }
+      iMod ("HinvC" with "HinvO") as "_".
+      set dst := ReplicaDurable clog ilog.
+      iMod ("HdurableC" $! dst with "[$Hclog $Hilog]") as "Hdurable".
+      by iIntros "!> %Hcontra".
+    }
+    (* Case: Write succeeded. Update the logical state and re-establish invariant. *)
+    iDestruct "Hfile" as "[Hfile %Hencilog']".
+    iNamed "HinvO".
+    iDestruct (big_sepS_elem_of_acc with "Hgroups") as "[Hgroup HgroupsC]"; first apply Hgid.
+    iDestruct (big_sepS_elem_of_acc with "Hrgs") as "[Hrg HrgsC]"; first apply Hgid.
+    iDestruct (big_sepS_elem_of_acc with "Hrg") as "[Hrp HrgC]"; first apply Hrid.
+    (* First catching up the consistent log. *)
+    destruct Hcloga as [cmdsa ->].
+    iMod (replica_inv_execute with "Hclogalb Hclog Hilog Hgroup Hrp")
+      as "(Hclog & Hilog & Hgroup & Hrp)".
+    (* Then apply the validate transition. *)
+    (* ∅ is a placeholder for participant groups. *)
+    iMod (replica_inv_advance ts rank cid with "Hclog Hilog Hrp")
+      as "(Hclog & Hilog & Hrp & H)".
+    { apply Hexec. }
+    { rewrite /advance_requirement.
+      destruct ok; rewrite Hrankl.
+      { (* Case: Has heard from coordinator @rankl. *)
+        rewrite not_and_r in Hadvanced.
+        destruct Hadvanced as [? | Horder]; first done.
+        clear -Horder. word.
+      }
+      { (* Case: Has not heard from any coordinator. *)
+        clear -Hvrank. rewrite /valid_backup_rank in Hvrank. lia.
+      }
+    }
+    iDestruct "H" as "(_ & #Hvote & %ra & %pa & #Hpromise & %Hlastacp)".
+    (* Close the file, replica, and crash invariants. *)
+    iDestruct (replica_ilog_split with "Hilog") as "[Hilog Hilogfileinv]".
+    iMod "Hmask" as "_".
+    iMod ("HinvfileC" with "[Hfile Hilogfileinv]") as "_".
+    { iFrame "∗ #".
+      iPureIntro.
+      split.
+      { apply Forall_app_2; first apply Hvilog.
+        rewrite Forall_singleton.
+        simpl.
+        split.
+        { clear -Hlencloga HlsnaW. word. }
+        split; word.
+      }
+      { by rewrite Hlencloga -HlsnaW. }
+    }
+    iDestruct ("HgroupsC" with "Hgroup") as "Hgroups".
+    iDestruct ("HrgC" with "Hrp") as "Hrg".
+    iDestruct ("HrgsC" with "Hrg") as "Hrgs".
+    iMod ("HinvC" with "[$Htxnsys $Hkeys $Hgroups $Hrgs]") as "_".
+    set ilog' := ilog ++ _.
+    set dst := ReplicaDurable (clog ++ cmdsa) ilog'.
+    iMod ("HdurableC" $! dst with "[$Hclog $Hilog]") as "Hdurable".
+    iIntros "!> _".
+
+    (*@     // Check whether the transaction has validated.                     @*)
+    (*@     pwrs, vd := rp.prepm[ts]                                            @*)
+    (*@                                                                         @*)
+    wp_apply (wp_Replica__validated with "Hcpm").
+    iIntros (pwrsP vd) "[Hcpm #Hpwrs]".
+    wp_pures.
+
+    (*@     // Return the last accepted prepare decision.                       @*)
+    (*@     return pp, vd, pwrs, tulip.REPLICA_OK                               @*)
+    (*@ }                                                                       @*)
+    iAssert ([∗ map] t ↦ ps ∈ init_psm ts psm, fast_proposal_witness γ gid rid t ps)%I
+      as "#Hfpw'".
+    { rewrite /init_psm.
+      destruct (psm !! ts) as [ps |] eqn:Hps; first done.
+      iApply big_sepM_insert_2; last done.
+      rewrite /fast_proposal_witness /=.
+      iNamed "Hpromise".
+      iFrame "Hlb".
+      iPureIntro.
+      rewrite /last_accepted_decision Hps in Hlastacp.
+      by destruct Hlastacp as [-> ->].
+    }
+    iClear "Hfpw".
+    iAssert (own_replica rp gid rid γ α)%I with "[-HΦ]" as "Hrp".
+    { iFrame "∗ # %".
+      iPureIntro.
+      split.
+      { rewrite /init_psm.
+        destruct (psm !! uint.nat tsW) as [p' |] eqn:Hpsmts.
+        { apply elem_of_dom_2 in Hpsmts.
+          rewrite dom_insert_L.
+          clear -Hpsmts Hdompsmrkm.
+          set_solver.
+        }
+        { rewrite 2!dom_insert_L.
+          clear -Hdompsmrkm.
+          set_solver.
+        }
+      }
+      split; first done.
+      rewrite merge_clog_ilog_snoc_ilog; last done.
+      split.
+      { rewrite Forall_forall.
+        intros [n c] Hilog. simpl.
+        apply elem_of_app in Hilog as [Hilog | Hnewc].
+        { rewrite Forall_forall in Hvicmds. by specialize (Hvicmds _ Hilog). }
+        rewrite elem_of_list_singleton in Hnewc.
+        by inv Hnewc.
+      }
+      { by rewrite /execute_cmds foldl_snoc execute_cmds_unfold Hexec /=. }
+    }
+    rewrite /last_accepted_decision in Hlastacp.
+    iNamed "Hpromise".
+    destruct vd eqn:Hvd; last first.
+    { iModIntro.
+      iApply ("HΦ" $! (ranka, pdec) _ _ ReplicaOK ∅). simpl.
+      destruct ex.
+      { rewrite Hex /= in Hlastacp.
+        iFrame "Hrp".
+        iSplit; last done.
+        inv Hlastacp as [Heq].
+        rewrite Heq in Hp *.
+        iFrame "# %".
+      }
+      { destruct Hex as (Hpsmts & Hranka & Hpdec).
+        rewrite Hpsmts in Hlastacp.
+        iFrame "Hrp".
+        iSplit; last done.
+        inv Hlastacp as [Heq].
+        rewrite Heq in Hp *.
+        iFrame "# %".
+      }
+    }
+    iDestruct "Hpwrs" as (pwrs) "[Hpwrs %Hpwrs]".
+    iDestruct (big_sepS_elem_of with "Hrpvds") as "Hvd".
+    { apply elem_of_dom_2 in Hpwrs. apply Hpwrs. }
+    iDestruct (big_sepM_lookup with "Hsafetpwrs") as "Hsafepwrs".
+    { apply Hpwrs. }
+    iApply ("HΦ" $! (ranka, pdec) _ _ ReplicaOK pwrs). simpl.
+    destruct ex.
+    { rewrite Hex /= in Hlastacp.
+      inv Hlastacp as [Heq].
+      rewrite Heq in Hp *.
+      by iFrame "∗ # %".
+    }
+    { destruct Hex as (Hpsmts & Hranka & Hpdec).
+      rewrite Hpsmts in Hlastacp.
+      inv Hlastacp as [Heq].
+      rewrite Heq in Hp *.
+      by iFrame "∗ # %".
+    }
+  Qed.
+
+End program.
